Assert macro

theories/examples/assert.v
@@ -8,7 +8,6 @@ From cap_machine Require Import logrel addr_reg_sample fundamental rules proofmo
 
 Section Assert.
   Context {Σ:gFunctors} {memg:memG Σ} {regg:regG Σ}
-          {nainv: logrel_na_invs Σ}
           `{MP: MachineParameters}.
 
   (* assert (r4 == r5) *)
@@ -37,82 +36,126 @@ Section Assert.
   *)
 
   Definition assert_inv (b a_flag e : Addr) : iProp Σ :=
-    (∃ cap_addr,
-       codefrag b assert_subroutine_instrs ∗
+    ( codefrag b assert_subroutine_instrs ∗
+      (∃ cap_addr,
        ⌜(b + length assert_subroutine_instrs)%a = Some cap_addr⌝ ∗
        ⌜(cap_addr + 1)%a = Some a_flag⌝ ∗
        ⌜(a_flag + 1)%a = Some e⌝ ∗
-       cap_addr ↦ₐ WCap RW a_flag e a_flag).
+       cap_addr ↦ₐ WCap RW a_flag e a_flag)).
 
-  Lemma assert_subroutine_spec b a_flag e cont n1 n2 flag N E φ :
+
+  Ltac fact :=
+    match goal with
+    | h : @ContiguousRegion _ ?a (Z.of_nat (@Datatypes.length _ ?code))
+      |- context [(@environments.Esnoc _ _ (INamed "Hprog") (@codefrag _ _ ?a ?code))]
+      => match goal with
+        | h: SubBounds ?b ?e ?a
+               (?a ^+ (Z.of_nat (@Datatypes.length _ ?code)))%a
+          |- context [(@environments.Esnoc _ _ _ ((_, PC) ↦ᵣ WCap _ ?b ?e _))]
+          => idtac
+        | _ => codefrag_facts "Hprog"
+        end
+    | _ => codefrag_facts "Hprog"
+    end.
+
+  Lemma assert_subroutine_spec i b a_flag e cont n1 n2 flag N E φ :
     ↑N ⊆ E →
-    (  na_inv logrel_nais N (assert_inv b a_flag e)
-     ∗ na_own logrel_nais E
-     ∗ PC ↦ᵣ WCap RX b e b
-     ∗ r_t0 ↦ᵣ cont
-     ∗ r_t4 ↦ᵣ WInt n1
-     ∗ r_t5 ↦ᵣ WInt n2
+    (  inv N (assert_inv b a_flag e)
+     ∗ (i,PC) ↦ᵣ WCap RX b e b
+     ∗ (i,r_t0) ↦ᵣ cont
+     ∗ (i,r_t4) ↦ᵣ WInt n1
+     ∗ (i,r_t5) ↦ᵣ WInt n2
      ∗ a_flag ↦ₐ WInt flag
-     ∗ ▷ (na_own logrel_nais E
-          ∗ PC ↦ᵣ updatePcPerm cont
-          ∗ r_t0 ↦ᵣ cont
-          ∗ r_t4 ↦ᵣ WInt 0
-          ∗ r_t5 ↦ᵣ WInt 0
+     ∗ ▷ ((i,PC) ↦ᵣ updatePcPerm cont
+          ∗ (i,r_t0) ↦ᵣ cont
+          ∗ (i,r_t4) ↦ᵣ WInt 0
+          ∗ (i, r_t5) ↦ᵣ WInt 0
           ∗ a_flag ↦ₐ WInt (if (n1 =? n2)%Z then flag else 1%Z)
-          -∗ WP Seq (Instr Executable) {{ φ }})
-     ⊢ WP Seq (Instr Executable) {{ φ }})%I.
+          -∗ WP (i, Seq (Instr Executable)) @ E {{ φ }})
+     ⊢ WP (i, Seq (Instr Executable)) @ E{{ φ }})%I.
   Proof.
-    iIntros (HNE) "(#Hinv & Hna & HPC & Hr0 & Hr1 & Hr2 & Hflag & Hφ)".
-    iMod (na_inv_acc with "Hinv Hna") as "(>Hassert & Hna & Hinv_close)"; auto.
-    iDestruct "Hassert" as (cap_addr) "(Hprog & %Hcap & %Hflag & %He & Hcap)".
-    rewrite /assert_subroutine_instrs. codefrag_facts "Hprog".
-    assert (SubBounds b e b (b ^+ length assert_subroutine_instrs)%a) by solve_addr.
-    do 3 iInstr "Hprog".
+    iIntros (HNE) "(#Hinv & HPC & Hr0 & Hr1 & Hr2 & Hflag & Hφ)".
+    iDestruct (inv_split_l with "Hinv") as "Hinv_code".
+
+    wp_instr.
+    iInv "Hinv" as ">[Hprog Hassert]" "Hcls".
+    iDestruct "Hassert" as (cap_addr) "(%Hcap & %Hflag & %He & Hcap)".
+    rewrite /assert_subroutine_instrs.
+    fact.
+    assert (SubBounds b e b (b ^+ length assert_subroutine_instrs)%a) by
+      solve_addr.
+    iInstr "Hprog".
+    (iMod ("Hcls" with "[$Hprog Hcap]") as "_" ;[| iModIntro ; wp_pure]).
+    { iNext ; iExists _ ; eauto. }
+    do 2 iInstr_inv "Hinv_code".
+
     destruct (decide (n1 = n2)).
     { (* n1 = n2 *)
       subst n2. rewrite (_: n1 - n1 = 0)%Z; last lia.
-      iGo "Hprog".
-      iMod ("Hinv_close" with "[Hprog Hcap $Hna]") as "Hna".
-      { iExists _. iNext. iFrame. iPureIntro. repeat split; solve_addr. }
+      repeat (iInstr_inv "Hinv_code").
       iApply "Hφ". iFrame. rewrite Z.eqb_refl //. }
     { (* n1 ≠ n2 *)
-      iInstr "Hprog". { assert (n1 - n2 ≠ 0)%Z by lia. congruence. }
-      iInstr "Hprog". rewrite (_: (b ^+ 13)%a = cap_addr). 2: solve_addr.
-      iInstr "Hprog". solve_addr.
-      iInstr "Hprog". solve_addr.
-      iGo "Hprog".
-      iMod ("Hinv_close" with "[Hprog Hcap $Hna]") as "Hna".
-      { iExists _. iNext. iFrame. iPureIntro. repeat split; solve_addr. }
+      iInstr_inv "Hinv_code". { assert (n1 - n2 ≠ 0)%Z by lia. congruence. }
+      iInstr_inv "Hinv_code". rewrite (_: (b ^+ 13)%a = cap_addr). 2: solve_addr .
+
+      (* Load *)
+      wp_instr.
+      iInv "Hinv" as ">[Hprog Hassert]" "Hcls".
+      iDestruct "Hassert" as (cap_addr') "(%Hcap' & %Hflag' & _ & Hcap)".
+      rewrite <- Hflag' in Hflag ; rewrite Hcap' in Hcap. simplify_eq.
+      rewrite /assert_subroutine_instrs.
+      iInstr "Hprog".
+      solve_addr.
+      (iMod ("Hcls" with "[$Hprog Hcap]") as "_" ;[| iModIntro ; wp_pure]).
+      { iNext ; iExists _ ; eauto. }
+
+      (* Store *)
+      wp_instr.
+      iInv "Hinv" as ">[Hprog Hassert]" "Hcls".
+      iDestruct "Hassert" as (cap_addr') "(%Hcap'' & %Hflag'' & _ & Hcap)".
+      rewrite <- Hflag'' in Hflag' ; rewrite Hcap'' in Hcap'. simplify_eq.
+      rewrite /assert_subroutine_instrs.
+      iInstr "Hprog".
+      solve_addr.
+      (iMod ("Hcls" with "[$Hprog Hcap]") as "_" ;[| iModIntro ; wp_pure]).
+      { iNext ; iExists _ ; eauto. }
+
+      repeat (iInstr_inv "Hinv_code").
       iApply "Hφ". iFrame. rewrite (_: (n1 =? n2)%Z = false) //.
       by apply Z.eqb_neq. }
   Qed.
 
-  Lemma assert_success_spec b a_flag e cont n1 n2 N E φ :
+  Lemma assert_success_spec i b a_flag e cont n1 n2 N E φ :
     ↑N ⊆ E →
     n1 = n2 →
-    (  na_inv logrel_nais N (assert_inv b a_flag e)
-     ∗ na_own logrel_nais E
-     ∗ PC ↦ᵣ WCap RX b e b
-     ∗ r_t0 ↦ᵣ cont
-     ∗ r_t4 ↦ᵣ WInt n1
-     ∗ r_t5 ↦ᵣ WInt n2
-     ∗ ▷ (na_own logrel_nais E
-          ∗ PC ↦ᵣ updatePcPerm cont
-          ∗ r_t0 ↦ᵣ cont
-          ∗ r_t4 ↦ᵣ WInt 0
-          ∗ r_t5 ↦ᵣ WInt 0
-          -∗ WP Seq (Instr Executable) {{ φ }})
-     ⊢ WP Seq (Instr Executable) {{ φ }})%I.
+    (  inv N (assert_inv b a_flag e)
+     ∗ (i, PC) ↦ᵣ WCap RX b e b
+     ∗ (i, r_t0) ↦ᵣ cont
+     ∗ (i, r_t4) ↦ᵣ WInt n1
+     ∗ (i, r_t5) ↦ᵣ WInt n2
+     ∗ ▷ ((i, PC) ↦ᵣ updatePcPerm cont
+          ∗ (i, r_t0) ↦ᵣ cont
+          ∗ (i, r_t4) ↦ᵣ WInt 0
+          ∗ (i, r_t5) ↦ᵣ WInt 0
+          -∗ WP (i, Seq (Instr Executable)) @ E{{ φ }})
+     ⊢ WP (i, Seq (Instr Executable)) @ E{{ φ }})%I.
   Proof.
-    iIntros (HNE Heq) "(#Hinv & Hna & HPC & Hr0 & Hr1 & Hr2 & Hφ)".
-    iMod (na_inv_acc with "Hinv Hna") as "(>Hassert & Hna & Hinv_close)"; auto.
-    iDestruct "Hassert" as (cap_addr) "(Hprog & %Hcap & %Hflag & %He & Hcap)".
-    rewrite /assert_subroutine_instrs. codefrag_facts "Hprog".
-    assert (SubBounds b e b (b ^+ length assert_subroutine_instrs)%a) by solve_addr.
-    do 3 iInstr "Hprog". rewrite (_: n1 - n2 = 0)%Z; last lia.
-    iGo "Hprog".
-    iMod ("Hinv_close" with "[Hprog Hcap $Hna]") as "Hna".
-    { iExists _. iNext. iFrame. iPureIntro. repeat split; solve_addr. }
+    iIntros (HNE Heq) "(#Hinv & HPC & Hr0 & Hr1 & Hr2 & Hφ)".
+    iDestruct (inv_split_l with "Hinv") as "Hinv_code".
+
+    wp_instr.
+    iInv "Hinv" as ">[Hprog Hassert]" "Hcls".
+    iDestruct "Hassert" as (cap_addr) "(%Hcap & %Hflag & %He & Hcap)".
+    rewrite /assert_subroutine_instrs.
+    fact.
+    assert (SubBounds b e b (b ^+ length assert_subroutine_instrs)%a) by
+      solve_addr.
+    iInstr "Hprog".
+    (iMod ("Hcls" with "[$Hprog Hcap]") as "_" ;[| iModIntro ; wp_pure]).
+    { iNext ; iExists _ ; eauto. }
+    do 2 iInstr_inv "Hinv_code".
+    rewrite (_: n1 - n2 = 0)%Z; last lia.
+    repeat iInstr_inv "Hinv_code".
     iApply "Hφ". iFrame.
   Qed.
 
